LeanMove/Typing.lean
@@ -16,5 +16,5 @@
 
 import LeanMove.Typing.TypeChecking
 import LeanMove.Typing.TypeSoundness
-import LeanMove.Typing.Algorithmic.TypeCheckingAlgorithmic
+import LeanMove.Typing.Algorithmic.AlgorithmicTypeChecking
 import LeanMove.Typing.Algorithmic.AlgorithmicTypingSoundness
